# Assignment 02
## 1
$$(AB)_{m\times p}C_{p\times q} = D_{m \times q}$$ $$A_{m\times n}(BC)_{n\times q}= D'_{m\times q}$$
Moreover,
$$D_{ij} = \sum_{k=1}^{p}(AB)_{ik}C_{kj}=\sum_{k=1}^{p}\sum_{q=1}^nA_{iq}B_{qk}C_{kj}=\sum_{q=1}^nA_{iq}\sum_{k=1}^{p}B_{qk}C_{kj}= \sum_{q=1}^{n}A_{iq}(BC)_{qj}=D_{ij}'$$
Hence $$D = D'.
\tag*□$$



## 2
$$[ A(B+C) ]_{ij} = \sum_{k=1}^n A_{ik}(B+C)_{kj} =\sum_{k=1}^n A_{ik}(B_{kj}+C_{kj}) = \sum_{k=1}^n A_{ik}B_{kj} + \sum_{k=1}^n A_{ik}C_{kj} = (AB)_{ij} + (AC)_{ij} = (AB + AC)_{ij}. $$
Therefore $$A(B+C) = AB+AC.\tag*□$$



## 3
###(a)
$$A^2 = \begin{bmatrix}
   1 & 0 & 0 \\
   0 & 1 & 0 \\
   0 & 0 & 1
\end{bmatrix}$$
$$A^3 = \begin{bmatrix}
   1 & 0 & 0 \\
   0 & 0 & 1 \\
   0 & 1 & 0
\end{bmatrix}$$
$$A^4 = \begin{bmatrix}
   1 & 0 & 0 \\
   0 & 1 & 0 \\
   0 & 0 & 1
\end{bmatrix}$$

###(b)
$$A^k=
\begin{cases}
\begin{bmatrix}
   1 & 0 & 0 \\
   0 & 0 & 1 \\
   0 & 1 & 0
\end{bmatrix} &\text{if } k \text{ is odd，}\\\\
\begin{bmatrix}
   1 & 0 & 0 \\
   0 & 1 & 0 \\
   0 & 0 & 1
\end{bmatrix} &\text{if } k \text{ is even.}
\end{cases}$$



## 4
Suppose $A_{n\times n},B_{n\times n}.$
If $A,B$ both invertible, then $A^{-1},B^{-1}$ both exist, and that $$(B^{-1}A^{-1})AB=AB(B^{-1}A^{-1})=I.$$Therefore $$A,B \text{ both invertible} \implies AB \text{ invertible.} $$ On the other hand, if $AB$ is invertible, suppose first $B$ is not invertible. Then $\exist x_B \neq0\  \text{s.t.} $$$\ Bx_B = 0.$$ Choosing $x = x_B \neq 0,$ $$(AB)x = A(Bx)=A\cdot0=0,$$ which implies $AB$ is not invertible, a contradiction. Hence $B$ is invertible.
Next, suppose $A$ is not invertible. Then $\exist x_A \neq0\  \text{s.t.} $$$ Ax_A = 0.$$Since $B$ is invertible, choosing $x = B^{-1}x^A \neq 0,$ $$(AB)x = A(BB^{-1})x_A=Ax_A=0,$$ a contradiction. Hence $A$ must also  be invertible. We proved
$$AB \text{ invertible} \iff A,B\text{ both invertible}.$$Then, if $M = A_{n\times n}B_{n\times n}C_{n\times n},$
$$M \text{ invertible} \iff  A(BC)\text{ invertible} \iff A,BC \text{ both invertible} \iff A,B,C \text{ all invertible}.\tag*□$$



## 5
### (a)
$$
\begin{aligned}
   1+ab&=3 \\
   4+a&=5
\end{aligned}
\implies a=1, b=2.
$$

### (b)
$$
\begin{aligned}
   1+ab&=1 \\
   a+b&=b \\
\end{aligned}
\implies a=0, b \text{ is free.}
$$

## 6
### (i)
$$
\left[
   \begin{array}{c|}
      1 & 2 & 3 \\
            \hline
      4 & 5 & 6 \\
      7 & 8 & 9
   \end{array}
\right]
\ \ \ \ \ \ 
\left[
   \begin{array}{c|}
   1 & 2 & 3 \\
   4 & 5 & 6 \\
   \hline
   7 & 8 & 9
   \end{array}
\right]
\ \ \ \ \ \ 
\left[
   \begin{array}{cc|}
   1 & 2 & 3 \\
      \hline
   4 & 5 & 6 \\
   7 & 8 & 9
   \end{array}
\right]
\ \ \ \ \ \ 
\left[
   \begin{array}{cc|}
   1 & 2 & 3 \\
   4 & 5 & 6 \\
   \hline
   7 & 8 & 9
   \end{array}
\right]$$

###(ii)
$$
\left[
   \begin{array}{c|c|}
   1 & 0 & 5 \\
   4 & 6 & 1 \\
   7 & 9 & 3
   \end{array}
\right]
$$

###(iii)
$$
\left[
   \begin{array}{ccc}
   1 & 0 & 5 \\
   \hline
   4 & 6 & 1 \\
   \hline
   7 & 9 & 3
   \end{array}
\right]
$$

## 7
###(a)
True. Suppose the $i$-th row of $A_{4\times 4}$ is of zeros. Then $\vec y = \left[y_1\ y_2\ y_3 \ y_4
   \right]$ with $y_i \neq 0$ and $y_j = 0\  \forall j \neq i$ satisfies $$
   \vec y A = \sum_{n=1}^4 y_n\vec a_n = \vec 0,
   $$ where $\vec a_n$ is the $n$-th row of $A$. Hence $A$ is not invertible.
###(b)
True. By definition if $A$ is invertible, $\exists A^{-1} \ \text{s.t.} $ $$A A^{-1}=A^{-1}A=I, $$ which, by definition implies $A = (A^{-1})^{-1}.$ Hence $A^{-1}$ is invertible.
###(c)
True. Suppose $A$ is not invertible, then $\exists x \neq 0 \ \text{s.t.}$$$Ax = 0.$$Taking the transpose,$$
\vec y A^T = \vec0
$$ where $\vec y = x^T \neq \vec 0,$ which implies $A^T $ is not invertible, a contradiction.
## 8
$$
\left[
   \begin{array}{ccc}
   2 & c & c \\
   c & c & c \\
   8 & 7 & c
   \end{array}
\right]
\xrightarrow{E_{12}E_{31}}
\left[
   \begin{array}{ccc}
   2-c & 0 & 0 \\
   c & c & c \\
   0 & 7-4c & -3c
   \end{array}
\right]
\xrightarrow[c\notin \{0,2\}]{E_{32}E_{21}}
\left[
   \begin{array}{ccc}
   2-c & 0 & 0 \\
   0 & c & c \\
   0 & 0 & c-7
   \end{array}
\right]
$$If and only if $c \in \{0,2,7\}, \exists$ row of the reduced matrix consisting solely of zeros, and the matrix is not invertible.
##9
$$
\left[
   \begin{array}{ccc}
   1 & \lambda & 0 \\
   1 & 1 & 1 \\
   0 & 0 & 1
   \end{array}
\right]
\xrightarrow{E_{23}E_{21}}
\left[
   \begin{array}{ccc}
   1 & \lambda & 0 \\
   0 & 1-\lambda & 0 \\
   0 & 0 & 1
   \end{array}
\right]
$$
If and only if $\lambda = 1, \exists$ row of the reduced matrix consisting solely of zeros, and the matrix is not invertible. Hence the matrix is invertible if and only if $\lambda \neq 1$.
##10
###(a)
$$
\left[
   \begin{array}{ccc|c}
   1 & 2 & 2 &&&\\
   3 & 7 & 9 &&I&\\
   -1 & -4 & -7&&&
   \end{array}
\right]
\xrightarrow{E_{32}E_{31}E_{21}}
\left[
   \begin{array}{ccc|c}
   1 & 2 & 2 &1&0&0\\
   0 & 1 & 3 &-3&1&0\\
   0 & 0 & 1& -5&2&1
   \end{array}
\right]
\xrightarrow{E_{12}E_{13}E_{23}}
\left[
   \begin{array}{ccc|c}
    &  &  &-13&6&4\\
    & I &  &12&-5&-3\\
    &  & & -5&2&1
   \end{array}
\right]
$$
###(b)
$$
\left[
   \begin{array}{ccc|c}
   1 & 1 & 1 &&&\\
   3 & 5 & 4 &&I&\\
   3 & 6 & 5&&&
   \end{array}
\right]
\xrightarrow{E_{32}E_{31}E_{21}}
\left[
   \begin{array}{ccc|c}
   1 & 1 & 1 &1&0&0\\
   0 & 2 & 1 &-3&1&0\\
   0 & 0 & 1/2&3/2&-3/2&1
   \end{array}
\right]
\xrightarrow{E_{12}E_{13}E_{23}}
\left[
   \begin{array}{ccc|c}
    &  &  &1&1&-1\\
    & I &  &-3&2&-1\\
    &  & & 3&-3&2
   \end{array}
\right]
$$
## 11
The system is non-singular if and only if $a\neq 0, a\neq b, b\neq c ,c\neq d.$
$$
A\overset{L}{\rightarrow}
\left[
   \begin{array}{cccc}
      a&a&a&a\\
        &b-a&b-a&b-a\\
       &&c-b&c-b\\
      \large0&&&d-c
   \end{array}
\right]
$$

where $$L=\left[
\begin{array}{cccc}
      1&&&\large{0}\\
        0&1&&\\
       0&0 &1&\\
      0& 0&-1&1
   \end{array}
\right]
\left[
   \begin{array}{cccc}
      1&&&\large{0}\\
        0&1&\\
       0&-1&1&\\
      0& -1&0&1
   \end{array}
\right]
\left[
   \begin{array}{cccc}
      1&&&\large{0}\\
        -1&1&&\\
       -1&0 &1&\\
      -1 & 0&0&1
   \end{array}
\right].$$

Hence$$
$$$$
A=
\underbrace{\left[
   \begin{array}{cccc}
      1&&&\large{0}\\
        1&1&&\\
       1&1&1&\\
      1& 1&1&1
   \end{array}
\right]}_{\tilde{L}\ =\ L^{-1}}\ 
\underbrace{
\left[
   \begin{array}{cccc}
      a&a&a&a\\
        &b-a&b-a&b-a\\
       &&c-b&c-b\\
      \large0&&&d-c
   \end{array}
\right]
}_{U}.
$$
## 12
$$
L=\left[
   \begin{array}{cccc}
      1&&&\large0\\
        1&1&&\\
       -3& 3&1&\\
      5& -1&-3&1
   \end{array}
\right], U = \left[
   \begin{array}{cccc}
      3&3&1&-4\\
        &2&-2&1\\
       & &5&1\\
      \large0& &&3
   \end{array}
\right].
$$Let $y=Ux, Ly=b.$
First solve for $y$ using forward substitution.
$$
\left[
   \begin{array}{cccc|c}
      1&&&\large0 &5\\
        1&1&&&5\\
       -3& 3&1&&-5\\
      5& -1&-3&1&-5
   \end{array}
\right]\implies
y=\left[
   \begin{array}{c}
      5\\
        0\\
       10\\
      0
   \end{array}
\right].
$$Then solve for $x$ using backward substitution.
$$
\left[
   \begin{array}{cccc|c}
      3&3&1&-4&5\\
        &2&-2&1&0\\
       & &5&1&10\\
      \large0& &&3&0
   \end{array}
\right]\implies
x=\left[
   \begin{array}{c}
      -1\\
        2\\
       2\\
      0
   \end{array}
\right].
$$
##13
###(a)
$$
\begin{aligned}
(I-uv^T)(I+\frac{uv^T}{1-v^Tu})
&=I+\frac{uv^T}{1-v^Tu}-uv^T-\frac{(uv^T)^2}{1-v^Tu}\\
&=I+\frac{\cancel{uv^T}-(uv^T)^2\cancel{-uv^T}+v^Tu\cdot uv^T}{1-v^Tu}\\
&=I+\frac{v^Tu\cdot uv^T-(uv^T)^2}{1-v^Tu}\tag{∗}
\end{aligned}
$$
Note that $(v^Tu\cdot uv^T)_{ij} = \sum_{x=1}^nv_xu_xu_iv_j=\sum_{x=1}^n(uv^T)_{ix}(uv^T)_{xj}=
[(uv^T)^2]_{ij}.$
Hence$$v^Tu\cdot uv^T-(uv^T)^2=O\tag{∗∗},$$and$$(∗)=I\implies M^{-1}=I+\frac{uv^T}{1-v^Tu}.$$

###(b)
$$
\begin{aligned}
(A-uv^T)(A^{-1}+\frac{A^{-1}uv^TA^{-1}}{1-v^TA^{-1}u})
&=
I+\frac{uv^TA^{-1}}{1-v^TA^{-1}u}-uv^TA^{-1}-\frac{(uv^TA^{-1})^2}{1-v^TA^{-1}u}\\
&=
I+\frac{\tilde{v}^Tu\cdot u\tilde{v}^T-(u\tilde{v}^T)^2}{1-\tilde{v}^Tu}
\end{aligned}
$$where $
\tilde{v} = (A^{-1})^Tv.
$ Using $(∗∗),$ a similar argument to $(b)$ implies that $$M^{-1}=A^{-1}+\frac{A^{-1}uv^TA^{-1}}{1-v^TA^{-1}u}.$$
###(c)
$$
\begin{aligned}
(I_n-UV)[I_n+U(I_m-VU)^{-1}V]
&=
I_n-UV+U(I_m-VU)^{-1}V-UVU(I_m-VU)^{-1}V\\
&=
I_n+U[(I_m-VU)^{-1}-VU(I_m-VU)^{-1}-I_m]V\\
&=
I_n+U[(I_m-VU)(I_m-VU)^{-1}-I_m]V
\\&=
I_n+U[I_m-I_m]V
\\&=I_n.
\end{aligned}
$$Hence$$M^{-1}=I_n+U(I_m-VU)^{-1}V.$$
###(d)
$$
\begin{aligned}
&(A-UW^{-1}V)[A^{-1}+A^{-1}U(W-VA^{-1}U)^{-1}VA^{-1}]\\
=&\ 
I_n-UW^{-1}VA^{-1}+U(W-VA^{-1}U)^{-1}VA^{-1}-UW^{-1}VA^{-1}U(W-VA^{-1}U)^{-1}VA^{-1}\\
=&\ 
I_n+U[(W-VA^{-1}U)^{-1}-W^{-1}VA^{-1}U(W-VA^{-1}U)^{-1}-W^{-1}]VA^{-1}\\
=&\ 
I_n+U[W^{-1}W(I_m-W^{-1}VA^{-1}U)(W-VA^{-1}U)^{-1}-W^{-1}]VA^{-1}
\\=&\ 
I_n+U[W^{-1}-W^{-1}]VA^{-1}
\\=&\ I_n.
\end{aligned}
$$Hence$$M^{-1}=A^{-1}+A^{-1}U(W-VA^{-1}U)^{-1}VA^{-1}.$$
##14
$(a), (c).$
##15
$$
\begin{aligned}
(AB)^{*}&=[(AB)^T]^{-1}\\
&=(B^TA^T)^{-1}\\
&=(A^T)^{-1}(B^T)^{-1}\\
&=A^*B^*.
\end{aligned}
$$
## 16
```julia
julia> using LinearAlgebra
```
###(a)
```julia {cmd="C:/Users/chen1/AppData/Local/Julia-1.1.1/bin/julia.exe"}

julia> res_norm_1 = norm(A * x1 - b)
2.541731896800047e-14
```
###(b)
```julia
julia> res_norm_2 = norm(A * x2 - b)
3.617300165427831e-14
```

##17
###(a)
```julia {cmd="C:/Users/chen1/AppData/Local/Julia-1.1.1/bin/julia.exe"}
julia> @time A\b
  1.722943 seconds (3.48 M allocations: 197.092 MiB, 3.80% gc time)
```
###(b)
```julia
julia> @time L\b
  0.005796 seconds (5 allocations: 15.906 KiB)
```

###(c)
The matrix $L$ is lower triangular while entries of $A$ are all non-zero.

$\text{Hypothesis:}$ Julia is solving the system using LU-decomposition.

##18
```julia
julia> using LinearAlgebra
```
###(a)
```julia
julia> norm(A * (B * C) - (A * B) * C) # Associativity
2.493235635302362e-14
```
###(b)
```julia
julia> norm(A * (B + C) - (A * B + A * C)) # Distributivity
7.32410687763558e-15
```
###(c)
```julia
julia> norm(A * B - B * A) # Noncommutativity
7.827281228408319
```
###(d)
```julia
julia> Ã = [A1 A2; A3 A4] # Blocks of A

julia> B̃ = [B1 B2; B3 B4] # Blocks of B

julia> norm(A * B - Ã * B̃) # Block Mult.
0.0
```
###(e)
```julia
julia> norm(inv(A * B) - inv(B) * inv(A)) # Properties of Inverse
3.5961261080715424e-13
```
##(19)
###(a)
```julia
julia> L, U, p = lu(A)
LU{Float64,Array{Float64,2}}
L factor:
10×10 Array{Float64,2}:
 1.0        0.0       0.0        …   0.0       0.0       0.0
 0.467841   1.0       0.0            0.0       0.0       0.0
 0.812289  -0.909545  1.0            0.0       0.0       0.0
 ⋮                               ⋱
 0.236137   0.640994  0.0606518     -0.554904  1.0       0.0
 0.647666  -0.162007  0.104964      -0.639265  0.978578  1.0
U factor:
10×10 Array{Float64,2}:
 0.805707  0.706994  0.656959  …  0.571168  0.104836   0.683771
 0.0       0.606948  0.517501     0.118659  0.817633   0.35018
 0.0       0.0       0.745954     0.580221  1.41523    0.278695
 ⋮                             ⋱
 0.0       0.0       0.0          0.0       1.53085   -0.324748
 0.0       0.0       0.0          0.0       0.0        0.171293
```
###(b)
####i.
Checked.
####ii.
```julia
julia> Ã = A[p,:] # Ã = PA

julia> norm(Ã - L * U)
5.933264665155888e-16
```
###(c)
```julia
function ldu(A)
    L, U, p = lu(A)
    D = diagm(0 => diag(U))
    U = inv(D) * U
    return L, D, U, p
end
```
###(d)
```julia
julia> L, D, U, p = ldu(A)

julia> norm(L * D * U - Ã)
8.266316859814843e-16
```
##20
###(a)

@import "j.png" {width="540" height="360" style="margin: 0 auto"}

The space character has the highest probability. This is reasonable because the space constantly occurs between each word.
###(b)

@import "pairwise (1).png" {width="575" height="520" style="margin: 0 auto"}

Some peaks in the conditional PMF: 
- The letter "q" is almost always followed by the letter "u," as in words "**qu**een" and "ac**qu**ire."
- The letter "v" is often succeeded by the letter "e," as in words "fi**ve**" and "**ve**st."
- The letter "y" usually ends a word, followed by a space, as in words "da**y**," "keenl**y**," etc.
###(c)
```julia
julia> randomSentence(ng, alphabet, 100, 0)
"s od keev ihdmluecu sr c eb b h u edrctilehia  shm pgetsfue  alcntod ett t daaysdfes oitecelinmkmfba"

julia> randomSentence(ng, alphabet, 100, 1)
" sizve t mes sevipere y phas f a dalonggeancororinus veary harvesllofouliny o tyod by rof alagamery "

julia> randomSentence(ng, alphabet, 100, 2)
"n topy ll ob saiddy yourawaidech askintentarieub the me mut what she we i fack has badodis ine of no"
```
*Comments*: The result is unsatisfactory. One main reason could be that the algorithm does not distinguish "characters" and "words." One way of improving the performance could be to include a dictionary of words allowed.