# MAT 4003 Assignment 1

## 1

Let $S=\{s_1,s_2,...s_{n+1}\}$ be an $(n+1)$-element subset of $\{1,2,...,2n+1\},$ where $1\le s_1\lt s_2\lt...\lt s_{n+1}\le2n+1$. If $S$ contains two consecutive integers $s, s+1,$ then $(s,s+1)=(s,1)=1.$ If $S$ does not contain two consecutive integers, then $1\le s_1\le s_2-2\le...\le s_{n+1}-2n\le 1.$ So $s_1=1.$ $(s_1,s_k)=(1,s_k)=1.$ In either case, $S$ contains a pair of relatively prime integers.$\ \ \Box$

## 2

Using EEA:

| $i$  | $r_i$   | $q_i$ | $x_i$   | $y_i$     |
| :--- | ------- | ----- | ------- | --------- |
| $-1$ | $43$    | -     | $1$     | $0$       |
| $0$  | $5$     | -     | $0$     | $1$       |
| $1$  | $3$     | $8$   | $1$     | $-8$      |
| $2$  | $2$     | $1$   | $-1$    | $9$       |
| $3$  | ==$1$== | $1$   | ==$2$== | ==$-17$== |
| $4$  | $0$     | -     | -       | -         |

$$
43(2)+5(-17)=(43,5)=1.
$$

Hence a particular solution to the original equation is
$$
x_0=500,y_0=-4250.
$$
And the complete solution is given by
$$
\{(x,y)\}=\{(500+1250k,-4250-10750k):k\in\Z\}.
$$

## 3

Set $p:=(a^m-1,a^n-1),d:=(m,n),m=sd,n=td.$ Then $(a^{d}-1)|((a^{d})^s-1)=a^{m}-1.$ Similarly $(a^{d}-1)|(a^{n}-1).$ Hence $(a^{d}-1)|p.$ Now by Bézout’s lemma we may write $d=mx+ny.$ WLOG assume $y\le0\le x.$ Then $\ p|(a^{mx}-1),(a^{-ny}-1).$ It follows that $p|(a^{mx}-1-a^d(a^{-ny}-1))=a^d-1.$ Therefore $p=2^d-1,$ or
$$
(a^m-1,a^n-1)=a^{(m,n)}-1.
$$
This in turn shows the equivalence:
$$
(a^m-1)|(a^n-1)\iff (a^m-1,a^n-1)=a^m-1=a^{(m,n)}-1\iff m|n.
$$

## 4

Proceed by strong induction on $n.$

Clearly $F_3=2>\phi.$ Now suppose $\forall n$ with $ 3\le n\le k$ we have $F_n>\phi^{n-2}.$ Then $F_{k+1}=F_{k}+F_{k-1}>\phi^{k-1}(\phi^{-2}+\phi^{-1})=\phi^{k-1}.$ Therefore,
$$
F_n\gt \phi^{n-2}\ \ \ \ \forall n\ge3.\ \  \Box
$$

## 5

Consider the Diophantine equation
$$
ax+by=ab-a-b.
$$
Note that $(x_0,y_0)=(b-1,-1)$ is a particular solution. Then by Theorem $(1.12)$ the complete solution set of the equation is given by
$$
\{(x,y)\}=\{((1-k)b-1,ka-1):k\in \Z\}.
$$
Now, for $x,y$ to both be nonnegative integers, one must have $(1-k)b\gt0$ and $ka\gt0.$ Equivalently $0\lt k\lt1.$ Therefore $x,y$ cannot both be nonnegative. That is, $ab-a-b$ is never a nonnegative integer linear combination of $a$ and $b.\ \ \Box$

