# MAT4003 Assignment 4

## 1

### (a)

Check in $\Z_{11}^*=\{1,2,3,...,10\}.$ There are $\phi(10)=4$ primitive roots. Since
$$
1^1\equiv
3^5\equiv
4^5\equiv
5^5\equiv
9^5\equiv
10^1\equiv1\pmod{11},
$$
the remaining four $\boxed{2,6,7,8}$ are all the primitive roots modulo $11.$

### (b)

Check in $\Z^*_{26}=\{1,3,5,7,9,11,15,17,19,21,23,25 \}.$ There are $\phi(\phi(26))=4$ primitive roots. Since
$$
1^1\equiv 3^3\equiv5^4\equiv9^3\equiv17^{6}\equiv21^4\equiv23^6\equiv25^1\equiv1\pmod{26},
$$
all primitive roots modulo $26$ are $\boxed{7,11,15,19.}$

## 2

### (a)

Write $22=2^111^1.$
$$
5^{22/2}=5^{11}\equiv22\not\equiv1\pmod{23}\\5^{22/11}\equiv5^{2}\equiv2\not\equiv1\pmod{23}.
$$
Therefore by p. $16$ of Lecture Notes of Section $4,$ $\boxed{5}$ is a primitive root of $23.$

### (b)

Note that $529=23^2.$ Since $5$ is a primitive root of $23,$ by Theorem $(4.12)$ either $5$ or $5+23=28$ must be a primitive root of $529.$ But $28^{22}\equiv 1\pmod{529}. $ Therefore $\boxed{5}$ is a primitive root of $529. $

## 3

**Claim.**  $\boxed{3}$ is such a number.

*Proof.*  $7^k:$ For $k=1$ we use the algorithm on p. $16$ of Lecture Notes of Section $4.$ Factor $6=2^13^1.$ Then $3^{6/2}\equiv 3^3\equiv6\not\equiv1\pmod{7};3^{6/3}\equiv3^2\equiv2\not\equiv1\pmod{7}.$ Therefore $3$ is a primitive root modulo $7.$ Similarly for $k=2,$ factor $48=2^43^1.$ Then $3^{48/2}\equiv3^{24}\equiv 22\not\equiv 1\pmod{49};3^{48/3}\equiv3^{16}\equiv3\not\equiv 1\pmod{49}.$ Thus $3$ is also a primitive root modulo $7^2.$ It follows from Theorem $(4.13)$ that $3$ is a primitive root modulo $p^k$ for all $k\ge1.$  

$2(7^k):$ Given any $k,$ we have proved that $3$ is a primitive root modulo $7^k.$ Now we want to show that $n:=\text{ord}_{2\cdot7^k}3=\phi(2\cdot7^k)=6\cdot7^{k-1}=\phi(7^k).$ 

Since $3$ is a primitive root of $7^k,$ we have $3^{\phi(7^k)}\equiv1\pmod{7^k}$ . Note that $3^{\phi(7^k)}\equiv1^{\phi(7^k)}\equiv1\pmod 2,$ and $(2,7^k)=1.$ It follows from CRT that $3^{\phi(7^k)}\equiv1\pmod{2\cdot7^k}.$ Therefore $n|\phi(7^k).$ Also by definition of $n,$ $3^n\equiv1\pmod {2\cdot7^k}.$ Again using CRT we have $3^n\equiv 1\pmod{7^k}.$ It follows that $\text{ord}_{7^k}3=\phi(7^k)|n.$ Finally $n=\phi(7^k).\ \ \ \Box$

## 4

Consider $p=4,$ which is not a prime. And let $f(x):=2x .$ Then the congruence
$$
f(x)=2x\equiv0\pmod4
$$
has *two* incongruent solutions, namely $x_{1,2}\equiv0,2\pmod4,$ instead of one.

## 5

Consider $x\in\{0,1,...p-1\}.$ Clearly $x\equiv1$ is not a solution to the congruence as $p-1\equiv-1\not\equiv0\pmod p.$ For $x\not\equiv1, $ congruence becomes

$$
\frac{x^{p-1}-1}{x-1}\equiv0\pmod p.
$$
Multiplying $x-1$ on both sides yields
$$
x^{p-1}\equiv1\pmod p,
$$
which by FLT is true for any $x$ coprime to $p.$ In this case $x\equiv 2,3,\cdots,p-1\pmod p.$ Therefore
$$
\boxed{x\equiv 2,3,\cdots,p-1\pmod p.}
$$

## 6

**Lemma.**  Let $p$ be prime with $p\ge5.$ If $g$ is a primitive root modulo $p,$ then $g^{-1}$ is a primitive root modulo $p$ with $g\not\equiv g^{-1}\pmod p.$ 

*Proof.*  We prove the contrapositive. Assume $g$ to be such that $g^{-1} $ is not a primitive root modulo $p$. Then $(g^{-1})^x\equiv1\pmod p$ for some $x\lt\phi(p)=p-1.$ But then $g^x\equiv (g^{-1})^xg^x\equiv (gg^{-1})^x\equiv1\pmod p.$ So $g$ is not a primitive root either. Moreover, if $g$ is a primitive root modulo $p,$ then since $p\ge 5,$ $|g|\not\equiv1\pmod p.$ It follows from Lemma $(2.12)$ that $g^2\not\equiv 1\pmod p,$ whence $ g\not\equiv g^{-1}\pmod p.\ \ \ \Box$

Let $p$ be prime with $p\ge5.$ There are precisely $\phi(\phi(p))=\phi(p-1)$ primitive roots modulo $p.$ It follows from Lemma above that those $\phi(p-1)$ roots can be partitioned into $\phi(p-1)/2$ pairs of mutual inverses modulo $p$.

## 7

Let $g$ be the primitive root modulo $p.$ Then $\{g,g^2,...g^{p-1}\}$ forms a reduced residue system modulo $p,$ by Theorem $(4.6).$ It follows that
$$
S_k=\sum_{n=1}^{p-1}n^k\equiv\sum_{n=1}^{p-1}g^{kn}\equiv \frac{g^k-g^{kp}}{1-g^k}\pmod{p}.\tag1\label1
$$
If $(p-1)|k,k=m(p-1),$
$$
S_k=\sum_{n=1}^{p-1}g^{(p-1)mn}\equiv  \sum_{n=1}^{p-1}1^{mn}\equiv p-1\equiv -1\pmod p.
$$
If $(p-1)\not|\ \ k,$ multiply $g^k-1$ on both sides of $(\ref1):$
$$
(g^k-1)S_k\equiv g^{kp}-g^k\equiv g^k-g^k\equiv0\pmod p.
$$
By Theorem $(4.1),$ $g^k\not\equiv 1\pmod p.$ Canceling $g^k-1$ gives $S_k\equiv 0 \pmod p.$ So
$$
S_k\equiv\begin{cases}
-1\ \ \ \ \ \text{  if }(p-1)|k,\\
0\ \ \ \ \ \ \ \  \text{  otherwise.}
\end{cases}
$$

## 8

Suppose some odd prime $p$ divides $2^m-1.$ Then $2^m\equiv1\pmod p.$ By Theorem $(4.1),\text{ord}_p2|m.$ Since $m$ is odd, $\text{ord}_p2$ is odd. Assume some odd prime $q$ divides $2^n+1.$ Then $2^n\equiv -1\pmod q.$ So $\text{ord}_q2\not|\ \ n.$ Also $2^{2n}\equiv1\pmod q.$ It follows that $\text{ord}_q2|2n,$ whence $\text{ord}_q2|2.$ So $\text{ord}_p2\neq \text{ord}_q2,$ and $p\neq q. $ Since $2^m-1$ and $2^n+1$ share no common prime factor, by FTA, $(2^m-1,2^n+1)=1.$

## 9

By Corollary $(4.2),\text{ord}_na=(n-1)|\phi(n).$ So $n-1\le\phi(n).$ But $\phi(n)\le n-1.$ Therefore $\phi(n)=n-1.$ $n$ is a prime.$\ \ \ \Box$

## 10

Denote the sequence as $(a_n).$ 

**Lemma 1.**  $(a_n)$ is periodic with period $p(p-1).$

*Proof.*  If $p|n,$ then $n\equiv0\pmod p,$
$$
(n+t)^{n+t}\equiv (0+0)^{n+t}\equiv 0^n\equiv n^n\pmod p.
$$
Assume $p\not |\ \ n.$ Then by FLT,
$$
(n+t)^{n+t}\equiv n^{n+p(p-1)}\equiv n^n1^p\equiv n^n\pmod p.\ \ \ \Box
$$
**Lemma 2.**  If $(a_n)$ is periodic with a period of $h,$ then $p(p-1)|h.$

*Proof.*  Write $h=pq+r,0\le r\lt p.$ Since $h$ is period, it holds for all $n\ge1 $
$$
(n+h)^{n+h}\equiv (n+r)^{n+h}\equiv  n^n\pmod p.
$$
Specifically, with $n:=p,$ we have
$$
r^{p+h}\equiv 0\pmod p.
$$
Since $r\lt p,$ $(r,p)=1.$ So $(r^{p+h-1},p)=1.$ Canceling $ r^{p+h-1}$ yields
$$
r\equiv0\pmod p\implies r=0\implies p|h.
$$
Also write $h=(p-1)q'+r',0\le r'\lt p-1.$ Then for all positive integers $n,k$
$$
(n+kh)^{n+kh}\equiv n^n\pmod p
$$
Let $k:=sp,s\ge1,$ we have
$$
n^{n+kh}\equiv n^n\pmod p\implies n^{kh}\equiv 1\pmod p.
$$
By FLT,
$$
n^{kh}\equiv [(n^{p-1})^{q'}n^{r'}]^k \equiv n^{kr'}\equiv n^{sr'} \equiv 1 \pmod p.
$$
Let $g$ be a primitive root of $p,$ and set $n:=g.$ Pick $s:=1$ and $2,$ we have
$$
g^{r'}\equiv g^{2r'}\equiv 1 \pmod p\implies 1\equiv 2 \pmod{\text{ord}_pg^{r'}}.
$$
Thus $\text{ord}_pg^{r'}=\frac{\text{ord}_pg}{(\text{ord}_pg,r')}=\frac{p-1}{(p-1,r')}=1.$ So $(p-1,r')=p-1.$ But $0\le r'\lt p-1,$ whence $r'=0,$ $(p-1)|h.$  Since $(p,p-1)=1,$ we have $p(p-1)|h.\ \ \ \Box$

Let $t:=p(p-1),$ and $s$ be the smallest period of $(a_n) .$ We wish to show $t=s.$ Since $t$ and $s$ are both periods of $(a_n),$ it holds for all $n\ge 1$ that $a_n=a_{n+xt+ys},$ where $xt+ys\gt0.$ By BÃ©zout's Lemma, $d:=(s,t)$ gives another period of $(a_n) .$ This forces $d=s,$ whence $s|t.$ By Lemma 2, we also have $t|s.$ Therefore $t=s.\ \ \ \Box$

## 11

**Lemma.**  Let $p$ be a prime. Then $x^2\equiv1\pmod {p^k}\iff x\equiv\pm1\pmod{p^k}.$

*Proof.*  Consider $f(x):=x^2-1\equiv 0\pmod p.$ By Lagrange's Theorem, there are exactly two solutions $x_{1,2}\equiv\pm 1\pmod p.$ $f'(x_1)\equiv2-1\equiv1\not\equiv0\pmod p.$ By Hensel's Lemma, $x_1\equiv 1\pmod p$ can be uniquely lifted to modulo $p^k.$ Now $f'(x_2)\equiv -3\pmod p.$ If $p\neq 3,$ then $f'(x_2)\not\equiv 0\pmod p.$ Again by Hensel's Lemma $x_2$ can be uniquely lifted to a root modulo $p^k.$ Suppose $p=3.$ To lift $x_2$ to modulo $3^2,$ we try $-1+3\equiv 2,-1+2\cdot3\equiv 5,-1+3\cdot3\equiv 8\pmod 9,$ with only $f(8)\equiv 0\pmod 9.$ In general, if $x\equiv 3^k-1\pmod {3^k}$ is the only solution to $f(x)\equiv0\pmod {3^k},$ then among the lifted $x,x+3^k,x+2\cdot3^k\pmod {3^{k+1}},$ 
$$
{f(x)\equiv 3^{2k}-2\cdot 3^k\equiv 3^k\pmod {3^{k+1}}\\f(x+3^k)\equiv f(2\cdot 3^k-1)\equiv -3^k\pmod {3^{k+1}}\\f(x+2\cdot 3^k)\equiv f(3^{k+1}-1)\equiv0\pmod {3^{k+1}}.}
$$
Only $f(3^{k+1}-1)\equiv 0\pmod {3^{k+1}}.$ By induction, $x_2$ is uniquely lifted to modulo $3^k.$ Thus for any odd prime $p, $ $f(x)\equiv 0\pmod{p^k}$ has exactly two solutions. Since $x\equiv \pm 1\pmod{p^k}$ are two solutions, the lemma follows.$\ \ \ \Box $

Let $g$ be a primitive root of $n.$ Then
$$
\prod_{i\in\Z_n^*}i\equiv \prod_{i=1}^{\phi(n)}g^i\equiv g^{1+2+\cdots+\phi(n)}\overset{n>2}=g^{\phi(n)/{2}}\pmod n.
$$
If $n=2$ or $4.$ Primitive roots are $1$ and $3$ respectively. We have
$$
\prod_{i\in\Z_2^*}i\equiv 1^1\equiv -1\pmod2;\prod_{i\in\Z_4^*}i\equiv 3^{2/2}\equiv -1\pmod4.
$$
If $n=p^k,$ where $p$ is an odd prime. Then $\phi(n)=p^{k}-p^{k-1},$
$$
\prod_{i\in\Z_n^*}i\equiv g^{\frac{p-1}{2}p^{k-1}}\pmod{p^k}.
$$
Since $(g^{(p-1)/2})^2\overset{\text{FLT}}\equiv 1\pmod{p^k},$ by Lemma, $g^{(p-1)/{2}}\equiv1$ or $-1\pmod {p^k}.$ But $g^{(p-1)/{2}}\equiv1$ is impossible as $g$ is a primitive root modulo $n.$ Therefore
$$
\prod_{i\in\Z_n^*}i\equiv(-1)^{p^{k-1}}\equiv -1 \pmod {p^k}.
$$
If $n=2p^k,$ where $p$ is any odd prime. Then $\phi(n)=\phi(p^k)=p^{k}-p^{k-1}.$ The argument coincides with the last case. Therefore in all cases,
$$
\prod_{i\in\Z_n^*}i\equiv -1 \pmod {n}.\ \ \ \Box
$$
