# DDA4250 Assignment 6

**CHEN Ang (118010009)** $\newcommand{\v}{\boldsymbol}$ $\newcommand{\b}{\mathbf}$ $\newcommand{\id}{\text{id}_\R}$



## Notation

- $\|\cdot\|:=\|\cdot\|_2$ is the L2 norm.
- $B_r(c):=\{x:\|x-c\|_2\le r\}$ is the closed ball with a radius $r$ and centered at $c$.



## 5.1.1

The statement is false. Suppose otherwise. Then take $\xi:=\theta\in B_r(ϑ)$ and denote $h:=\xi-ϑ=\theta-ϑ$. It follows that
$$
\|h-\gamma g(\xi)\|\le \varepsilon\|h\|
$$
Squaring,
$$
\|h-\gamma g(\xi)\|^2=\|h\|^2-2\gamma\langle h, g(\theta)\rangle+\gamma^2\|g(\theta)\|^2\le \varepsilon^2\|h\|^2
$$
Rearranging the inequality gives
$$
\begin{aligned}
\langle h, g(\theta)\rangle&\ge\frac{1-\varepsilon^2}{2\gamma}\|h\|^2+\frac\gamma2\|g(\theta)\|^2\\
&\ge \min\left\{\frac{1-\varepsilon^2}{2\gamma},\frac\gamma2\right\}(\|h\|^2+\|g(\theta)\|^2)\\
&\ge \min\left\{\frac{1-\varepsilon^2}{2\gamma},\frac\gamma2\right\}\max\left\{\|h\|^2,\|g(\theta)\|^2\right\}

\end{aligned}
$$
a contradiction.



## 5.1.2

Denote $g:=g(\theta),h:=\theta-ϑ$. It suffices to show that $\langle h,g\rangle\ge\frac12\max\{\|h\|^2,\|g\|^2\}$ implies $\|g\|\le 2\|h\|$. Indeed, if $\|g\|\gt 2\|h\|$,
$$
\langle h,g\rangle\le\|h\|\|g\|\lt \frac12 \|g\|^2= \frac12\max\{\|h\|^2,\|g\|^2\}
$$


## 5.1.3

By FTC,
$$
\begin{aligned}
f(ϑ+tv)-f(ϑ+sv)&=f\left[ϑ+sv+x(tv-sv)\right]_{x=0}^1\\
&=\int_{0}^1\nabla f\left[ϑ+sv+x(tv-sv)\right]\cdot (tv-sv)\ dx \\
&=\int_{0}^1\nabla f\left[ϑ+sv+x(tv-sv)\right]\cdot [x(tv-sv)]\frac1x\ dx \\
&=\int_{0}^1\nabla f\left[ϑ+sv+x(tv-sv)\right]\cdot [sv+[x(tv-sv)]\frac1x-sv]\ dx\\
&=\int_{0}^1\nabla f\left[ϑ+sv+x(tv-sv)\right]\cdot [sv+[x(tv-sv)]\frac1x-sv]\ dx






\end{aligned}
$$





$$
\begin{aligned}
f(ϑ+tv)-f(ϑ+sv)&=f(\vartheta+tv)-f(\vartheta)-(f(\theta))

\end{aligned}
$$







By lemma 4.2.8 it holds for all $\theta\in B_r(ϑ)$ that
$$
f(ϑ+tv)-f(ϑ)\ge\frac c2\|tv\|^2=\frac c2t^2\|v\|^2\\
f(ϑ+sv)-f(ϑ)\ge\frac c2\|sv\|^2=\frac c2s^2\|v\|^2\\
f(ϑ+tv-sv)-f(ϑ)\ge\frac c2\|tv-sv\|^2=\frac c2(t-s)^2\|v\|^2\\
$$

$$
\langle tv,\nabla f(ϑ+tv)\rangle\ge c\|tv\|^2=ct^2\|v\|^2\\
\langle sv,\nabla f(ϑ+sv)\rangle\ge c\|sv\|^2=cs^2\|v\|^2
$$
and
$$
f(ϑ+tv)-f(ϑ+sv)=(t-s)\nabla f(ϑ)\cdot v+(t^2-s^2)v^\top H_f(ϑ)v+\cdots\\
\ge c(t-s)\|v\|^2+(t)
$$


Differencing,
$$
\langle tv,\nabla f(ϑ+tv)-\langle sv,\nabla f(ϑ+sv)\ge 
$$


## 5.1.4

Let $\theta$ be arbitrary. Consider $tv=\theta-\vartheta$ and $sv=0$, i.e., $\vartheta+tv=\theta$ and $\vartheta+sv=\vartheta$. From the given,
$$
f(\theta)-f(\vartheta)=f(\vartheta+tv)-f(\vartheta+sv)\ge c(t^2-s^2)\|v\|^2=c\|t v\|^2=c\|\theta-\vartheta\|^2
$$
But by FTC
$$

$$